Foundation/Modal/Kripke/AxiomL.lean
@@ -1,0 +1,118 @@
+import Foundation.Vorspiel.BinaryRelations
+import Foundation.Modal.Kripke.FiniteFrame
+
+namespace LO.Modal
+
+open Formula.Kripke
+
+namespace Kripke
+
+abbrev TransitiveConverseWellFoundedFrameClass : FrameClass := { F | Transitive F.Rel ∧ ConverseWellFounded F.Rel }
+abbrev TransitiveIrreflexiveFiniteFrameClass : FiniteFrameClass := { F | Transitive F.Rel ∧ Irreflexive F.Rel }
+
+variable {F : Frame}
+
+lemma validate_L_of_trans_and_cwf (hTrans : Transitive F.Rel) (hCWF : ConverseWellFounded F.Rel) : F ⊧ (Axioms.L (.atom 0)) := by
+  rintro V w;
+  apply Satisfies.imp_def.mpr;
+  contrapose;
+  intro h;
+  obtain ⟨x, Rwx, h⟩ := by simpa using Satisfies.box_def.not.mp h;
+  obtain ⟨m, ⟨⟨rwm, hm⟩, hm₂⟩⟩ := hCWF.has_min ({ x | (F.Rel w x) ∧ ¬(Satisfies ⟨F, V⟩ x (.atom 0)) }) $ by use x; tauto;
+  replace hm₂ : ∀ x, w ≺ x → ¬Satisfies ⟨F, V⟩ x (.atom 0) → ¬m ≺ x := by simpa using hm₂;
+  apply Satisfies.box_def.not.mpr;
+  push_neg;
+  use m;
+  constructor;
+  . assumption;
+  . apply Satisfies.imp_def.not.mpr;
+    push_neg;
+    constructor;
+    . intro n rmn;
+      apply not_imp_not.mp $ hm₂ n (hTrans rwm rmn);
+      exact rmn;
+    . assumption;
+
+lemma trans_of_validate_L : F ⊧ (Axioms.L (.atom 0)) → Transitive F.Rel := by
+  contrapose;
+  intro hT;
+  obtain ⟨w, v, Rwv, u, Rvu, nRwu⟩ := by simpa [Transitive] using hT;
+  apply ValidOnFrame.not_of_exists_valuation_world;
+  use (λ w _ => w ≠ v ∧ w ≠ u), w;
+  apply Satisfies.imp_def.not.mpr;
+  push_neg;
+  constructor;
+  . intro x Rwx hx;
+    by_cases exv : x = v;
+    . subst x;
+      simpa using Satisfies.atom_def.mp $ @hx u Rvu;
+    . apply Satisfies.atom_def.mpr;
+      constructor;
+      . assumption;
+      . by_contra hC;
+        subst x;
+        contradiction;
+  . apply Satisfies.box_def.not.mpr;
+    push_neg;
+    use v;
+    constructor;
+    . assumption;
+    . simp [Semantics.Realize, Satisfies];
+
+lemma cwf_of_validate_L : F ⊧ (Axioms.L (.atom 0)) → ConverseWellFounded F.Rel := by
+  contrapose;
+  intro hCF;
+  obtain ⟨X, ⟨x, _⟩, hX₂⟩ := by simpa using ConverseWellFounded.iff_has_max.not.mp hCF;
+  apply ValidOnFrame.not_of_exists_valuation_world;
+  use (λ w _ => w ∉ X), x;
+  apply Satisfies.imp_def.not.mpr;
+  push_neg;
+  constructor;
+  . intro y Rxy;
+    by_cases hys : y ∈ X
+    . obtain ⟨z, _, Rxz⟩ := hX₂ y hys;
+      intro hy;
+      have : z ∉ X := by simpa using Satisfies.atom_def.mp $ hy z Rxz;
+      contradiction;
+    . intro _;
+      apply Satisfies.atom_def.mpr;
+      simpa;
+  . obtain ⟨y, _, _⟩ := hX₂ x (by assumption);
+    apply Satisfies.box_def.not.mpr;
+    push_neg;
+    use y;
+    constructor;
+    . assumption;
+    . simpa [Semantics.Realize, Satisfies];
+
+instance TransitiveConverseWellFoundedFrameClass.DefinedByL : TransitiveConverseWellFoundedFrameClass.DefinedByFormula (Axioms.L (.atom 0)) := ⟨by
+  intro F;
+  constructor;
+  . simpa using validate_L_of_trans_and_cwf;
+  . intro h;
+    constructor;
+    . apply trans_of_validate_L; simp_all;
+    . apply cwf_of_validate_L; simp_all;
+⟩
+
+instance TransitiveIrreflexiveFiniteFrameClass.DefinedByL : TransitiveIrreflexiveFiniteFrameClass.DefinedByFormula (Axioms.L (.atom 0)) := ⟨by
+  intro F;
+  constructor;
+  . rintro ⟨hTrans, hIrrefl⟩ φ ⟨_, rfl⟩;
+    apply validate_L_of_trans_and_cwf;
+    . assumption;
+    . apply Finite.converseWellFounded_of_trans_irrefl'
+      . exact F.world_finite;
+      . assumption;
+      . assumption;
+  . intro h;
+    refine ⟨?_, ?_⟩;
+    . apply trans_of_validate_L;
+      simpa using h;
+    . intro w;
+      simpa using ConverseWellFounded.iff_has_max.mp (cwf_of_validate_L (by simpa using h)) {w} (by simp);
+⟩
+
+end Kripke
+
+end LO.Modal
