Foundation/Modal/Kripke/Hilbert/K.lean
@@ -1,0 +1,40 @@
+import Foundation.Modal.Hilbert.K
+import Foundation.Modal.Kripke.Hilbert.Soundness
+import Foundation.Modal.Kripke.Completeness
+import Foundation.Modal.Kripke.Filteration
+import Foundation.Modal.Kripke.FiniteFrame
+
+namespace LO.Modal
+
+open Kripke
+
+namespace Hilbert.K
+
+instance Kripke.sound : Sound (Hilbert.K) AllFrameClass := inferInstance
+
+instance : System.Consistent (Hilbert.K) := Hilbert.consistent_of_FrameClass AllFrameClass
+
+instance : Kripke.Canonical (Hilbert.K) (AllFrameClass) := ⟨by trivial⟩
+
+instance Kripke.CompleteAll : Complete (Hilbert.K) (AllFrameClass) := inferInstance
+
+instance Kripke.CompleteAllFinite : Complete (Hilbert.K) (AllFiniteFrameClass) := ⟨by
+  intro φ hp;
+  apply Kripke.CompleteAll.complete;
+  intro F _ V x;
+  let M : Kripke.Model := ⟨F, V⟩;
+  let FM := coarsestFilterationModel M ↑φ.subformulas;
+
+  apply filteration FM (coarsestFilterationModel.filterOf) (by aesop) |>.mpr;
+  apply hp (by
+    suffices Finite (FilterEqvQuotient M φ.subformulas) by
+      use ⟨FM.toFrame⟩;
+      simp [FiniteFrameClass.toFrameClass];
+    apply FilterEqvQuotient.finite;
+    simp;
+  ) FM.Val
+⟩
+
+end Hilbert.K
+
+end LO.Modal
