Foundation/Modal/Kripke/Hilbert/KTB.lean
@@ -1,0 +1,49 @@
+import Foundation.Modal.Kripke.Hilbert.Geach
+import Foundation.Modal.Kripke.Filteration
+import Foundation.Modal.Kripke.FiniteFrame
+
+namespace LO.Modal
+
+open Kripke
+open Geachean
+
+abbrev Kripke.ReflexiveSymmetricFrameClass : FrameClass := { F | Reflexive F ∧ Symmetric F }
+abbrev Kripke.ReflexiveSymmetricFiniteFrameClass : FiniteFrameClass := { F | Reflexive F.Rel ∧ Symmetric F.Rel }
+
+namespace Hilbert.KTB
+
+instance Kripke.consistent : System.Consistent (Hilbert.KTB) := by
+  convert Hilbert.Geach.Kripke.Consistent (G := {⟨0, 0, 1, 0⟩, ⟨0, 1, 0, 1⟩});
+  exact eq_Geach;
+
+instance Kripke.complete : Complete (Hilbert.KTB) (Kripke.ReflexiveSymmetricFrameClass) := by
+  convert Hilbert.Geach.Kripke.Complete (G := {⟨0, 0, 1, 0⟩, ⟨0, 1, 0, 1⟩});
+  . exact eq_Geach;
+  . unfold ReflexiveSymmetricFrameClass MultiGeacheanConfluentFrameClass MultiGeachean;
+    simp [Geachean.reflexive_def, Geachean.symmetric_def];
+
+instance Kripke.finiteComplete : Complete (Hilbert.KTB) (ReflexiveSymmetricFiniteFrameClass) := ⟨by
+  intro φ hp;
+  apply Kripke.complete.complete;
+  intro F ⟨F_refl, F_symm⟩ V x;
+  let M : Kripke.Model := ⟨F, V⟩;
+  let FM := finestFilterationModel M φ.subformulas;
+  apply filteration FM (finestFilterationModel.filterOf) (by aesop) |>.mpr;
+  apply hp (by
+    suffices Finite (FilterEqvQuotient M φ.subformulas) by
+      simp only [FiniteFrameClass.toFrameClass, ReflexiveSymmetricFiniteFrameClass, Set.mem_image, Set.mem_setOf_eq];
+      use ⟨FM.toFrame⟩;
+      refine ⟨⟨?_, ?_⟩, ?_⟩;
+      . apply reflexive_filterOf_of_reflexive (finestFilterationModel.filterOf);
+        exact F_refl;
+      . apply finestFilterationModel.symmetric_of_symmetric;
+        exact F_symm;
+      . rfl;
+    apply FilterEqvQuotient.finite;
+    simp;
+  ) FM.Val
+⟩
+
+end Hilbert.KTB
+
+end LO.Modal
