Foundation/Modal/Kripke/Hilbert/S4Dot3.lean
@@ -1,0 +1,15 @@
+import Foundation.Modal.Kripke.Hilbert.Geach
+import Foundation.Modal.Kripke.AxiomDot3
+
+namespace LO.Modal
+
+open Kripke
+open Geachean
+
+abbrev Kripke.ReflexiveTransitiveConnectedFrameClass : FrameClass := { F | Reflexive F ∧ Transitive F ∧ Connected F }
+
+namespace Hilbert.S4Dot3
+
+end Hilbert.S4Dot3
+
+end LO.Modal
