Foundation/Modal/Kripke/Hilbert/Soundness.lean
@@ -1,0 +1,125 @@
+import Foundation.Modal.Hilbert.Basic
+import Foundation.Modal.Kripke.FiniteFrame
+
+namespace LO.Modal
+
+open Kripke
+open Formula
+open Formula.Kripke
+
+namespace Kripke.Hilbert
+
+variable {H : Hilbert ℕ} {Γ : Set (Formula ℕ)} {φ : Formula ℕ}
+
+
+section
+
+variable {C : Kripke.FrameClass}
+
+lemma soundness_of_FrameClass_definedBy_axiomInstances [defined : C.DefinedBy H.axiomInstances] : H ⊢! φ → C ⊧ φ := by
+  intro hφ F hF;
+  induction hφ using Hilbert.Deduction.rec! with
+  | maxm h =>
+    obtain ⟨ψ, h, ⟨s, rfl⟩⟩ := h;
+    apply defined.defines F |>.mp hF (ψ⟦s⟧);
+    use ψ;
+    constructor;
+    . assumption;
+    . use s;
+  | mdp ihpq ihp => exact ValidOnFrame.mdp ihpq ihp;
+  | nec ih => exact ValidOnFrame.nec ih;
+  | imply₁ => exact ValidOnFrame.imply₁;
+  | imply₂ => exact ValidOnFrame.imply₂;
+  | ec => exact ValidOnFrame.elimContra;
+
+instance [defs : C.DefinedBy H.axioms] : C.DefinedBy H.axiomInstances := ⟨by
+  intro F;
+  constructor;
+  . rintro hF φ ⟨ψ, hψ, ⟨s, rfl⟩⟩;
+    exact ValidOnFrame.subst $ defs.defines F |>.mp hF ψ hψ;
+  . intro h;
+    apply defs.defines F |>.mpr;
+    intro φ hφ;
+    apply h;
+    use φ;
+    constructor;
+    . assumption;
+    . use .id;
+      simp;
+⟩
+
+instance [C.DefinedBy H.axioms] : Sound H C := ⟨fun {_} => soundness_of_FrameClass_definedBy_axiomInstances⟩
+
+lemma consistent_of_FrameClass_aux [nonempty : C.IsNonempty] [sound : Sound H C] : H ⊬ ⊥ := by
+  apply not_imp_not.mpr sound.sound;
+  apply ValidOnFrameClass.not_of_exists_frame;
+  obtain ⟨F, hF⟩ := nonempty;
+  use F;
+  constructor;
+  . assumption;
+  . simp;
+
+lemma consistent_of_FrameClass (C : Kripke.FrameClass) [C.IsNonempty] [Sound H C] : System.Consistent H := by
+  apply System.Consistent.of_unprovable;
+  exact consistent_of_FrameClass_aux (C := C);
+
+end
+
+
+section
+
+variable {C : Kripke.FiniteFrameClass}
+
+lemma soundness_of_FiniteFrameClass_definedBy_axiomInstances [defined : C.DefinedBy H.axiomInstances] : H ⊢! φ → C ⊧ φ := by
+  rintro hφ _ ⟨F, ⟨hF, rfl⟩⟩;
+  induction hφ using Hilbert.Deduction.rec! with
+  | maxm h =>
+    obtain ⟨ψ, h, ⟨s, rfl⟩⟩ := h;
+    apply defined.defines F |>.mp hF (ψ⟦s⟧);
+    use ψ;
+    constructor;
+    . assumption;
+    . use s;
+  | mdp ihpq ihp => exact ValidOnFrame.mdp ihpq ihp;
+  | nec ih => exact ValidOnFrame.nec ih;
+  | imply₁ => exact ValidOnFrame.imply₁;
+  | imply₂ => exact ValidOnFrame.imply₂;
+  | ec => exact ValidOnFrame.elimContra;
+
+instance [defs : C.DefinedBy H.axioms] : C.DefinedBy H.axiomInstances := ⟨by
+  intro F;
+  constructor;
+  . rintro hF φ ⟨ψ, hψ, ⟨s, rfl⟩⟩;
+    exact ValidOnFrame.subst $ defs.defines F |>.mp hF ψ hψ;
+  . intro h;
+    apply defs.defines F |>.mpr;
+    intro φ hφ;
+    apply h;
+    use φ;
+    constructor;
+    . assumption;
+    . use .id;
+      simp;
+⟩
+
+instance [C.DefinedBy H.axioms] : Sound H C := ⟨fun {_} => soundness_of_FiniteFrameClass_definedBy_axiomInstances⟩
+
+lemma consistent_of_FiniteFrameClass_aux [nonempty : C.IsNonempty] [sound : Sound H C] : H ⊬ ⊥ := by
+  apply not_imp_not.mpr sound.sound;
+  apply ValidOnFrameClass.not_of_exists_frame;
+  obtain ⟨F, hF⟩ := nonempty;
+  use F.toFrame;
+  constructor;
+  . use F;
+  . simp;
+
+lemma consistent_of_FiniteFrameClass (C : Kripke.FiniteFrameClass) [C.IsNonempty] [Sound H C] : System.Consistent H := by
+  apply System.Consistent.of_unprovable;
+  exact consistent_of_FiniteFrameClass_aux (C := C);
+
+end
+
+
+end Kripke.Hilbert
+
+end LO.Modal
