Foundation/Modal/Kripke/Hilbert/Ver.lean
@@ -1,0 +1,35 @@
+import Foundation.Modal.Kripke.AxiomVer
+import Foundation.Modal.Kripke.Hilbert.Soundness
+import Foundation.Modal.Hilbert.WellKnown
+
+namespace LO.Modal
+
+open Kripke
+
+namespace Kripke
+
+open System
+
+variable {S} [System (Formula ℕ) S]
+variable {𝓢 : S} [System.Consistent 𝓢]
+
+instance [System.Ver 𝓢] : Canonical 𝓢 IsolatedFrameClass := ⟨by
+  intro x y Rxy;
+  have : (canonicalModel 𝓢) ⊧ □⊥ := iff_valid_on_canonicalModel_deducible.mpr axiomVer!
+  exact this x _ Rxy;
+⟩
+
+end Kripke
+
+
+namespace Hilbert.Ver
+
+instance Kripke.Consistent : System.Consistent (Hilbert.Ver) :=
+  haveI := FrameClass.definedBy_with_axiomK IsolatedFrameClass.DefinedByAxiomVer
+  Kripke.Hilbert.consistent_of_FrameClass IsolatedFrameClass
+
+instance Kripke.Complete : Complete (Hilbert.Ver) IsolatedFrameClass := inferInstance
+
+end Hilbert.Ver
+
+end LO.Modal
