Foundation/Modal/Kripke/Preservation.lean
@@ -1,0 +1,332 @@
+import Foundation.Modal.Kripke.Closure
+
+namespace LO.Modal
+
+namespace Kripke
+
+open Formula.Kripke
+
+section Bisimulation
+
+structure Model.Bisimulation (M₁ M₂ : Kripke.Model) where
+  toRel : Rel M₁.World M₂.World
+  atomic {x₁ : M₁.World} {x₂ : M₂.World} {a : ℕ} : toRel x₁ x₂ → ((M₁ x₁ a) ↔ (M₂ x₂ a))
+  forth {x₁ y₁ : M₁.World} {x₂ : M₂.World} : toRel x₁ x₂ → x₁ ≺ y₁ → ∃ y₂ : M₂.World, toRel y₁ y₂ ∧ x₂ ≺ y₂
+  back {x₁ : M₁.World} {x₂ y₂ : M₂.World} : toRel x₁ x₂ → x₂ ≺ y₂ → ∃ y₁ : M₁.World, toRel y₁ y₂ ∧ x₁ ≺ y₁
+
+infix:80 " ⇄ " => Model.Bisimulation
+
+instance : CoeFun (Model.Bisimulation M₁ M₂) (λ _ => M₁.World → M₂.World → Prop) := ⟨λ bi => bi.toRel⟩
+
+end Bisimulation
+
+
+section ModalEquivalent
+
+def ModalEquivalent {M₁ M₂ : Model} (w₁ : M₁.World) (w₂ : M₂.World) : Prop := ∀ {φ}, w₁ ⊧ φ ↔ w₂ ⊧ φ
+infix:50 " ↭ " => ModalEquivalent
+
+lemma modal_equivalent_of_bisimilar (Bi : M₁ ⇄ M₂) (bisx : Bi x₁ x₂) : x₁ ↭ x₂ := by
+  intro φ;
+  induction φ using Formula.rec' generalizing x₁ x₂ with
+  | hatom a => exact Bi.atomic bisx;
+  | himp φ ψ ihp ihq =>
+    constructor;
+    . intro hpq hp;
+      exact ihq bisx |>.mp $ hpq $ ihp bisx |>.mpr hp;
+    . intro hpq hp;
+      exact ihq bisx |>.mpr $ hpq $ ihp bisx |>.mp hp;
+  | hbox φ ih =>
+    constructor;
+    . intro h y₂ rx₂y₂;
+      obtain ⟨y₁, ⟨bisy, rx₁y₁⟩⟩ := Bi.back bisx rx₂y₂;
+      exact ih bisy |>.mp (h _ rx₁y₁);
+    . intro h y₁ rx₁y₁;
+      obtain ⟨y₂, ⟨bisy, rx₂y₂⟩⟩ := Bi.forth bisx rx₁y₁;
+      exact ih bisy |>.mpr (h _ rx₂y₂);
+  | _ => simp_all;
+
+end ModalEquivalent
+
+
+section PseudoEpimorphism
+
+structure Frame.PseudoEpimorphism (F₁ F₂ : Kripke.Frame) where
+  toFun : F₁.World → F₂.World
+  forth {x y : F₁.World} : x ≺ y → toFun x ≺ toFun y
+  back {w : F₁.World} {v : F₂.World} : toFun w ≺ v → ∃ u, toFun u = v ∧ w ≺ u
+
+infix:80 " →ₚ " => Frame.PseudoEpimorphism
+
+instance : CoeFun (Frame.PseudoEpimorphism F₁ F₂) (λ _ => F₁.World → F₂.World) := ⟨λ f => f.toFun⟩
+
+namespace Frame.PseudoEpimorphism
+
+variable {F F₁ F₂ F₃ : Kripke.Frame}
+
+def id : F →ₚ F where
+  toFun := _root_.id
+  forth := by simp;
+  back := by simp;
+
+def TransitiveClosure (f : F₁ →ₚ F₂) (F₂_trans : Transitive F₂) : F₁^+ →ₚ F₂ where
+  toFun := f.toFun
+  forth := by
+    intro x y hxy;
+    induction hxy with
+    | single hxy => exact f.forth hxy;
+    | @tail z y _ Rzy Rxz =>
+      replace Rzy := f.forth Rzy;
+      exact F₂_trans Rxz Rzy;
+  back := by
+    intro x w hxw;
+    obtain ⟨u, ⟨rfl, hxu⟩⟩ := f.back hxw;
+    use u;
+    constructor;
+    . rfl;
+    . exact Frame.RelTransGen.single hxu;
+
+def comp (f : F₁ →ₚ F₂) (g : F₂ →ₚ F₃) : F₁ →ₚ F₃ where
+  toFun := g ∘ f
+  forth := by
+    intro x y hxy;
+    exact g.forth $ f.forth hxy;
+  back := by
+    intro x w hxw;
+    obtain ⟨y, ⟨rfl, hxy⟩⟩ := g.back hxw;
+    obtain ⟨u, ⟨rfl, hfu⟩⟩ := f.back hxy;
+    use u;
+    constructor;
+    . simp_all;
+    . assumption;
+
+end Frame.PseudoEpimorphism
+
+
+structure Model.PseudoEpimorphism (M₁ M₂ : Kripke.Model) extends M₁.toFrame →ₚ M₂.toFrame where
+  atomic {w : M₁.World} : (M₁ w a) ↔ (M₂ (toFun w) a)
+
+infix:80 " →ₚ " => Model.PseudoEpimorphism
+
+instance : CoeFun (Model.PseudoEpimorphism M₁ M₂) (λ _ => M₁.World → M₂.World) := ⟨λ f => f.toFun⟩
+
+namespace Model.PseudoEpimorphism
+
+variable {M M₁ M₂ M₃ : Kripke.Model}
+
+def id : M →ₚ M where
+  toFun := _root_.id
+  forth := by simp;
+  back := by simp;
+  atomic := by simp;
+
+def ofAtomic (f : M₁.toFrame →ₚ M₂.toFrame) (atomic : ∀ {w a}, (M₁ w a) ↔ (M₂ (f w) a)) : M₁ →ₚ M₂ where
+  toFun := f
+  forth := f.forth
+  back := f.back
+  atomic := atomic
+
+def comp (f : M₁ →ₚ M₂) (g : M₂ →ₚ M₃) : M₁ →ₚ M₃ := ofAtomic (f.toPseudoEpimorphism.comp (g.toPseudoEpimorphism)) $ by
+  intro x φ;
+  constructor;
+  . intro h;
+    apply g.atomic.mp;
+    apply f.atomic.mp;
+    assumption;
+  . intro h;
+    apply f.atomic.mpr;
+    apply g.atomic.mpr;
+    assumption;
+
+def bisimulation (f : M₁ →ₚ M₂) : M₁ ⇄ M₂ where
+  toRel := Function.graph f
+  atomic := by
+    rintro x₁ x₂ a rfl;
+    constructor;
+    . apply f.atomic.mp;
+    . apply f.atomic.mpr;
+  forth := by
+    simp only [Function.graph_def, exists_eq_left', forall_eq'];
+    intro x₁ y₁ rx₁y₁;
+    exact f.forth rx₁y₁;
+  back := by
+    simp only [Function.graph_def];
+    rintro x₁ x₂ y₂ rfl rx₂y₂;
+    obtain ⟨y₁, ⟨rfl, _⟩⟩ := f.back rx₂y₂;
+    use y₁;
+
+lemma modal_equivalence (f : M₁ →ₚ M₂) (w : M₁.World) : w ↭ (f w) := by
+  apply modal_equivalent_of_bisimilar $ Model.PseudoEpimorphism.bisimulation f;
+  simp [Model.PseudoEpimorphism.bisimulation];
+
+end Model.PseudoEpimorphism
+
+
+variable {F₁ F₂ : Kripke.Frame} {M₁ M₂ : Kripke.Model}
+
+lemma validOnFrame_of_surjective_pseudoMorphism (f : F₁ →ₚ F₂) (f_surjective : Function.Surjective f) : F₁ ⊧ φ → F₂ ⊧ φ := by
+  contrapose;
+  intro h;
+  obtain ⟨V₂, w₂, h⟩ := ValidOnFrame.exists_valuation_world_of_not h;
+  obtain ⟨w₁, rfl⟩ := f_surjective w₂;
+
+  apply ValidOnFrame.not_of_exists_valuation_world;
+  let V₁ := λ w a => V₂ (f w) a;
+  use V₁, w₁;
+
+  exact Model.PseudoEpimorphism.modal_equivalence (M₁ := ⟨F₁, V₁⟩) (M₂ := ⟨F₂, V₂⟩) {
+    toFun := f,
+    forth := f.forth,
+    back := f.back,
+    atomic := by aesop;
+  } w₁ |>.not.mpr h;
+
+lemma theory_ValidOnFrame_of_surjective_pseudoMorphism (f : F₁ →ₚ F₂) (f_surjective : Function.Surjective f) : F₁ ⊧* T → F₂ ⊧* T := by
+  simp only [Semantics.realizeSet_iff];
+  intro h φ hp;
+  exact validOnFrame_of_surjective_pseudoMorphism f f_surjective (h hp);
+
+end PseudoEpimorphism
+
+
+def Frame.isRooted (F : Frame) (r : F.World) : Prop := ∀ w ≠ r, r ≺ w
+
+structure RootedFrame extends Kripke.Frame where
+  root : World
+  root_rooted : Frame.isRooted _ root
+  default := root
+
+
+section PointGenerated
+
+def Frame.PointGenerated (F : Kripke.Frame) (r : F.World) : Kripke.RootedFrame where
+  World := { w | w = r ∨ r ≺ w }
+  Rel x y := x.1 ≺ y.1
+  world_nonempty := ⟨r, by tauto⟩
+  root := ⟨r, by tauto⟩
+  root_rooted := by
+    rintro ⟨x, (rfl | hx)⟩;
+    . intro h; contradiction;
+    . intro _; exact hx;
+infix:100 "↾" => Frame.PointGenerated
+
+namespace Frame.PointGenerated
+
+variable {F : Kripke.Frame} {r : F.World}
+
+lemma rel_transitive (F_trans : Transitive F) : Transitive (F↾r).Rel := by
+  rintro ⟨x, (rfl | hx)⟩ ⟨y, (rfl | hy)⟩ ⟨z, (rfl | hz)⟩ hxy hyz;
+  all_goals aesop;
+
+lemma rel_irreflexive (F_irrefl : Irreflexive F) : Irreflexive (F↾r).Rel := by
+  rintro ⟨x, (rfl | hx)⟩ h;
+  all_goals aesop;
+
+lemma rel_universal (F_refl : Reflexive F) (F_eucl : Euclidean F) : Universal (F↾r).Rel := by
+  have F_symm := symm_of_refl_eucl F_refl F_eucl;
+  rintro ⟨x, (rfl | hx)⟩ ⟨y, (rfl | hy)⟩;
+  . apply F_refl;
+  . exact hy;
+  . exact F_symm hx;
+  . apply F_symm $ F_eucl hx hy;
+
+instance [Finite F.World] : Finite (F↾r).World := by
+  unfold Frame.PointGenerated;
+  apply Subtype.finite;
+
+instance [DecidableEq F.World] : DecidableEq (F↾r).World := by
+  apply Subtype.instDecidableEq (p := λ w => w = r ∨ r ≺ w);
+
+end Frame.PointGenerated
+
+
+structure RootedModel extends Kripke.Model, Kripke.RootedFrame where
+
+
+def Model.PointGenerated (M : Kripke.Model) (r : M.World) : Kripke.RootedModel :=
+  letI rF := M.toFrame↾r;
+  {
+    toFrame := rF.toFrame
+    Val := λ w a => M.Val w.1 a
+    root := rF |>.root
+    root_rooted := rF.root_rooted
+  }
+infix:100 "↾" => Model.PointGenerated
+
+namespace Model.PointGenerated
+
+variable {M : Kripke.Model}
+
+def bisimulation_of_trans (M_trans : Transitive M.Rel) (r : M.World) : (M↾r).toModel ⇄ M where
+  toRel x y := x.1 = y
+  atomic := by
+    rintro x y a rfl;
+    simp [Model.PointGenerated];
+  forth := by
+    rintro x₁ y₁ x₂ rfl Rx₂y₁;
+    use y₁.1;
+    constructor;
+    . simp;
+    . exact Rx₂y₁;
+  back := by
+    rintro ⟨x₁, (rfl | hx₁)⟩ x₂ y₂ rfl Rx₂y₂;
+    . use ⟨y₂, by right; exact Rx₂y₂⟩;
+      constructor;
+      . simp;
+      . exact Rx₂y₂;
+    . use ⟨y₂, ?h₂⟩;
+      constructor;
+      . simp;
+      . exact Rx₂y₂;
+      right;
+      exact M_trans hx₁ Rx₂y₂;
+
+lemma modal_equivalent_at_root (M_trans : Transitive M.toFrame) (r : M.World) : ModalEquivalent (M₁ := (M↾r).toModel) (M₂ := M) ⟨r, by simp⟩ r
+  := modal_equivalent_of_bisimilar (bisimulation_of_trans M_trans r) $ by simp [bisimulation_of_trans];
+
+end Model.PointGenerated
+
+end PointGenerated
+
+
+section Generation
+
+structure Frame.GeneratedSub (F₁ F₂ : Kripke.Frame) extends F₁ →ₚ F₂ where
+ monic : Function.Injective toFun
+
+infix:80 " ⊆ₚ " => Frame.GeneratedSub
+
+end Generation
+
+
+/-
+namespace Frame
+
+variable {F : Kripke.Frame} (x : F.World)
+
+def successors := { w | x ≺^* w }
+postfix:100 "↑*" => Frame.upward
+
+def immediate_successors := { w | x ≺ w }
+postfix:100 "↑¹" => Frame.immediate_successor
+
+def proper_immediate_successors := { w | x ≠ w ∧ x ≺ w }
+postfix:100 "↑" => Frame.proper_immediate_successor
+
+
+def predeccsors := { w | w ≺^* x }
+postfix:100 "↓*" => Frame.downward
+
+def immediate_predeccsors := { w | w ≺ x }
+postfix:100 "↓¹" => Frame.immediate_predeccsor
+
+def proper_immediate_predeccsors := { w | w ≠ x ∧ w ≺ x }
+postfix:100 "↓" => Frame.proper_immediate_predeccsors
+
+end Frame
+-/
+
+
+end Kripke
+
+end LO.Modal
